assignment 7ab, switch emebed_subst to a definition

Deduction.thy
@@ -40,4 +40,69 @@ lemma deduce_cut:
 proof(induction rule:deduce.induct)
 qed(auto intro:deduce.intros)
 
+(* assignment 7 *)
+datatype constraint =
+Constraint "msg list " "msg list " "msg " ( "((2_/|_)/} _) " [67,67,67]66)
+(* elements go from the first list to the second.
+they are popped from the head of the first list and are push to the top
+of the second one *)
+
+type_synonym system = "constraint list"
+
+(* (a) *)
+(* functions lifted to msg list get a postfix l
+functions lifted to constraints get a postfix c
+functions lifted to systems get a postfix s *)
+definition sapplyl::"subst_msg \<Rightarrow> msg list \<Rightarrow> msg list" where
+"sapplyl s l = map (sapply_msg s) l"
+definition sapplyc:: "subst_msg \<Rightarrow> constraint \<Rightarrow> constraint" where
+"sapplyc s c = (case c of  a|m}t \<Rightarrow> (sapplyl s a)|(sapplyl s m)}( sapply_msg s t))"
+definition sapplys:: "subst_msg \<Rightarrow> system \<Rightarrow> system" where
+"sapplys s cs = map (sapplyc s) cs"
+
+lemma sapplyc_scomp:"sapplyc (scomp_msg t s) c = sapplyc t (sapplyc s (c))"
+  apply(cases c)
+  apply(auto simp add:sapplyc_def sapplyl_def)
+    apply(simp_all add:sapply_msg_scomp_msg)
+  done
+
+definition fvl:: "msg list \<Rightarrow> var set" where
+"fvl l = (\<Union>m \<in> set l. fv_msg m)"
+definition fvc:: "constraint \<Rightarrow> var set" where
+"fvc c = (case c of a|m}t \<Rightarrow> (fvl a) \<union> (fvl m) \<union> (fv_msg t))"
+definition fvs:: "system \<Rightarrow> var set" where
+"fvs cs = (\<Union>c \<in> set cs. fvc c)"
+
+(* (b) *)
+(* solution set *)
+definition solved:: "constraint \<Rightarrow> bool" where
+"solved c = (case c of (m|a}t) \<Rightarrow> ((set m \<union> set a) \<turnstile> t))"
+
+definition sol:: "system \<Rightarrow> subst_msg set" where
+"sol cs = {s. (\<forall> c \<in> set cs. solved (sapplyc s c))}"
+
+lemma solE: "s \<in> sol cs \<Longrightarrow> ((\<And>c. c \<in> set cs \<Longrightarrow> solved (sapplyc s c)) \<Longrightarrow> P) \<Longrightarrow>P"
+  by(auto simp add:sol_def)
+
+lemma solI: "(\<And>c. c \<in> set cs \<Longrightarrow> solved (sapplyc s c)) \<Longrightarrow> s \<in> sol cs"
+  by(auto simp add:sol_def)
+
+(* lemmas *)
+
+lemma sol_concat: "sol(cs @ cs') = sol(cs) \<inter> sol(cs')"
+proof((rule equalityI;rule subsetI),rule IntI)
+qed(auto simp add:sol_def)
+
+lemma "sol_scomp": "t \<in> sol(sapplys s cs) \<Longrightarrow> (scomp_msg t s) \<in> sol(cs)"
+proof(rule solI, erule solE)
+  fix c
+  assume w:"c \<in> set cs"
+  assume x:"\<And>d. d \<in> set (sapplys s cs) \<Longrightarrow> solved (sapplyc t d)"
+  have "solved (sapplyc (scomp_msg t s) c) = solved (sapplyc t (sapplyc s c))" (is "_ = solved (sapplyc t (?d))")
+    by(simp add: sapplyc_scomp)
+  moreover have "?d \<in> set (sapplys s cs)" by(simp add:w sapplys_def)
+  ultimately show "solved (sapplyc (scomp_msg t s) c)"
+    by(simp add:x)
+qed
+
 end
